First working version

src/widget.lean
@@ -1,42 +1,53 @@
 import init.meta.widget.tactic_component
+import stactic
 
 section tac
-open tactic widget
+open tactic widget tactic.sudoku
 
 meta def list.iota' : ℕ → list ℕ :=
 list.map (λ n, n - 1) ∘ list.reverse ∘ list.iota
 
-meta def mk_table_entry (n m : ℕ) : tactic (html empty) :=
+meta def get_numbers (n m : ℕ) : list cell_data → list ℕ :=
+list.erase_dup ∘ list.filter_map
+  (λ cd : cell_data, if cd.row.1 = n ∧ cd.col.1 = m then some (
+    if cd.val.1 = 0 then 9 else cd.val.1) else none)
+
+meta def mk_table_entry (n m : ℕ) (cd : list cell_data) : tactic (html empty) :=
 do
   let attrs : list (attr empty) := [cn "bw2"],
   let attrs := if n % 3 = 0 then attrs ++ [cn "bt"] else attrs,
   let attrs := if m % 3 = 0 then attrs ++ [cn "bl"] else attrs,
   let attrs := if n % 3 = 2 then attrs ++ [cn "bb"] else attrs,
   let attrs := if m % 3 = 2 then attrs ++ [cn "br"] else attrs,
-  let s := if n ≤ 8 ∧ m ≤ 8 then "7" else "",
+  let ns := get_numbers n m cd,
+  let s : string := match ns with
+  | [] := ""
+  | (a::[]) := to_string a
+  | (a::as) := "💥"
+  end,
   return $ h "td" attrs [
     h "div" [cn "dt", cn "ba", cn "b--light-silver", cn "w3", cn "h3"] [
       h "p" [cn "dtc", cn "v-mid", cn "tc", cn "f2"] s
     ]
   ]
 
-meta def mk_table_row (n : ℕ) : tactic (html empty) :=
+meta def mk_table_row (n : ℕ) (cd : list cell_data) : tactic (html empty) :=
 do
-  a ← list.mmap (λ m, mk_table_entry n m) (list.iota' 9),
+  a ← list.mmap (λ m, mk_table_entry n m cd) (list.iota' 9),
   return $ h "tr" [] a
 
-meta def mk_table : tactic (html empty) :=
+meta def mk_table (cd : list cell_data) : tactic (html empty) :=
 do
-  a ← list.mmap (λ n, mk_table_row n) (list.iota' 9),
+  a ← list.mmap (λ n, mk_table_row n cd) (list.iota' 9),
   return $ h "table" [cn "collapse"] a
 
-meta def hello_world_tac : tactic (list (html empty)) :=
+meta def sudoku_widget : tactic (list (html empty)) :=
 do
+  s ← get_sudoku,
+  cd ← get_cell_data s,
   g ← local_context,
-  u ← mk_table,
-  return [h "p" [] format!"Hello world! There are {list.length g} hypotheses!",
-    u
-  ]
+  u ← mk_table cd,
+  return [u]
 
 end tac
 
@@ -44,52 +55,52 @@ section tc
 
 open widget
 
-meta def hello_world : tc unit empty :=
-tc.stateless $ λ _, hello_world_tac
+meta def sudoku_component : tc unit empty :=
+tc.stateless $ λ _, sudoku_widget
 
-meta def combined : tc unit empty :=
+meta def combined_component : tc unit empty :=
 tc.stateless $ λ _,
 do
   s ← tactic.read,
   return [
-    h "div" [] [html.of_component s (tc.to_component hello_world)],
+    h "div" [] [html.of_component s (tc.to_component sudoku_component)],
     h "hr" [] [],
     h "div" [] [html.of_component s tactic_state_widget]
   ]
 
 end tc
 
-@[reducible] meta def hello_world_exec := tactic
+@[reducible] meta def show_sudoku := tactic
 
 open tactic
 
 meta def copy_decl (d : declaration) : tactic unit :=
-add_decl $ d.update_name $ d.to_name.update_prefix `hello_world_exec.interactive
+add_decl $ d.update_name $ d.to_name.update_prefix `show_sudoku.interactive
 
 meta def copy_decls : tactic unit :=
 do env ← get_env,
   let ls := env.fold [] list.cons,
   ls.mmap' $ λ dec, when (dec.to_name.get_prefix = `tactic.interactive) (copy_decl dec)
 
-namespace hello_world_exec
+namespace show_sudoku
 
-meta def step {α : Type} (t : hello_world_exec α) : hello_world_exec unit :=
+meta def step {α : Type} (t : show_sudoku α) : show_sudoku unit :=
 t >> return ()
 
 meta def istep := @tactic.istep
 
-meta def save_info (p : pos) : hello_world_exec unit :=
+meta def save_info (p : pos) : show_sudoku unit :=
 do
   s ← tactic.read,
   tactic.save_info_thunk p (λ _, tactic_state.to_format s),
-  tactic.save_widget p (widget.tc.to_component combined)
+  tactic.save_widget p (widget.tc.to_component combined_component)
 
-end hello_world_exec
+end show_sudoku
 
 run_cmd copy_decls
 
 example (P Q : Prop) (i : P → Q) (j : P) : Q :=
-begin [hello_world_exec]
+begin [show_sudoku]
   apply i,
   have : true := trivial,
   exact j,
